Two tiers should work but normalization is still buggy

Phoas.v
@@ -25,119 +25,314 @@ Module Stlc(Import PF: GaloisField.GaloisField).
   Notation "<{{ e }}>" := e (e custom stlc_ty at level 99).
   Notation "( x )" := x (in custom stlc_ty, x at level 99).
   Notation "x" := x (in custom stlc_ty at level 0, x constr at level 0).  
-  Notation "S -> T" := (TArrow S T) (in custom stlc_ty at level 2, right associativity).
+  Notation "S -> T" := (TArrow S T)
+                         (in custom stlc_ty at level 2, right associativity).
   Notation "'Num'" := TNum (in custom stlc_ty at level 0).
   Notation "'Bool'" := TBool (in custom stlc_ty at level 0).
 
-  (** This is STLC PHOAS syntax [Term] without control flow,
-      it includes normalization by evaluation using reify/reflect as seen in Oliver Danvy et al.
-      As reification of Coq terms [if _ then _ else _] is impossible without
-      meta-programming, we develop a meta-language [IM] that reifies control-flow, then
-      commute with reify/reflect on STLC with our meta-language.
-      
-      We get the following commutative square for *reflect*
+  (** This is STLC PHOAS syntax with strong normalization *)
+  Fixpoint typeDenote(t: type): Type :=
+    match t with
+    | <{{ Bool }}> => bool
+    | <{{ Num }}> => Fp
+    | <{{ a -> b }}> => (typeDenote a) -> (typeDenote b)
+    end.
 
+  Section pterms.
+    Variable var: type -> Type.
 
-                                  ireflect
-      IM (Term typeDenote) t ----------------> IM typeDenote t
-             |                                       | 
-             |                                       |
-             |                                       |
-             v                    reflect            v
-          Term typeDenote t  -----------------> typeDenote t
-
-
-      And the following for *reify*
-      
-                        reify
-      typeDenote t  -------------> Term typeDenote t
-             |                             | 
-             | RET                         | RET
-             |                             |
-             v            ireify           v
-      IM typeDenote t  ----------------> IM (Term typeDenote) t
-   *)
-  Section vars.
-    (** This is how to get reflected Coq terms *)
-    Variable var : type -> Type.
-
-    Inductive Term: type -> Type :=
-    (* Constants *)
-    | NUM: Fp -> Term <{{ Num }}>
-    | BOOL: bool -> Term <{{ Bool }}>
+    Inductive PTerm : type -> Type :=
+    (* Pure *)
     (* Finite field arithmetic *)
-    | ADD: Term <{{ Num }}> -> Term <{{ Num }}> -> Term <{{ Num }}>
-    | SUB: Term <{{ Num }}> -> Term <{{ Num }}> -> Term <{{ Num }}>
-    | MUL: Term <{{ Num }}> -> Term <{{ Num }}> -> Term <{{ Num }}>
-    | DIV: Term <{{ Num }}> -> Term <{{ Num }}> -> Term <{{ Num }}>
+    | ADD: PTerm <{{ Num }}> -> PTerm <{{ Num }}> -> PTerm <{{ Num }}>
+    | SUB: PTerm <{{ Num }}> -> PTerm <{{ Num }}> -> PTerm <{{ Num }}>
+    | MUL: PTerm <{{ Num }}> -> PTerm <{{ Num }}> -> PTerm <{{ Num }}>
+    | DIV: PTerm <{{ Num }}> -> PTerm <{{ Num }}> -> PTerm <{{ Num }}>
+    | ITE: forall t, PTerm <{{ Bool }}> -> PTerm t -> PTerm t -> PTerm t
     (* Logical formulas *)
-    | EQ: Term <{{ Num }}> -> Term <{{ Num }}> -> Term <{{ Bool }}>
-    | AND: Term <{{ Bool }}> -> Term <{{ Bool }}> -> Term <{{ Bool }}>
-    | OR: Term <{{ Bool }}> -> Term <{{ Bool }}> -> Term <{{ Bool }}>
-    | NOT: Term <{{ Bool }}> -> Term <{{ Bool }}>
+    | EQ: PTerm <{{ Num }}> -> PTerm <{{ Num }}> -> PTerm <{{ Bool }}>
+    | AND: PTerm <{{ Bool }}> -> PTerm <{{ Bool }}> -> PTerm <{{ Bool }}>
+    | OR: PTerm <{{ Bool }}> -> PTerm <{{ Bool }}> -> PTerm <{{ Bool }}>
+    | NOT: PTerm <{{ Bool }}> -> PTerm <{{ Bool }}>
+    | L: forall a, LTerm a -> PTerm a
+    with LTerm: type -> Type :=
+    (* Constants *)
+    | NUM: Fp -> LTerm <{{ Num }}>
+    | BOOL: bool -> LTerm <{{ Bool }}>
     (* Lambda *)
-    | APP: forall a b, Term <{{ a -> b }}> -> Term a -> Term b
-    | VAR: forall a, var a -> Term a
-    | LAM: forall a b, (var a -> Term b) -> Term <{{ a ->  b }}>.
+    | APP: forall a b, LTerm <{{ a -> b }}> -> LTerm a -> LTerm b
+    | VAR: forall a, var a -> LTerm a
+    | LAM: forall a b, (var a -> LTerm b) -> LTerm <{{ a ->  b }}>
+    | P: forall a, PTerm a -> LTerm a.
 
-    Fixpoint typeDenote (t : type) : Set :=
-      match t with
-      | <{{ Bool }}> => bool
-      | <{{ Num }}> => Fp
-      | <{{ t1 -> t2 }}> => typeDenote t1 -> typeDenote t2
-      end.
-
-    (* Normalization via reify/reflect Danvy et al. *)
-    Class Nbe (t: type) := {
-      reify: typeDenote t -> Term t;
-      reflect: Term t -> typeDenote t
-                          }.
-
-    Instance Nbe_lam {a b: type} `{Nbe a} `{Nbe b}: Nbe <{{ a -> b }}> := {
-      reify v := LAM (fun x => reify (v (reflect (VAR x))));        
-      reflect e :=  fun x => reflect (APP e (reify x))
-                                                                        }.
-  End vars.
-
-  (** This is the metalanguage with if-then-else. I am defining another
-      [T: type -> Type] because I want to be able to reflect terms in stages,
-      first in Terms and then in IM.
-
-      This allows us to have both Terms and IM Terms reified,
-      using [IM (Term typeDenote) t] and object terms reflected while
-      meta-terms remain reified using [IM typeDenote t]. This is a handy
-      trick for staged compilation of meta-languages! *)
-  Section mvars.
-
-    Variable T: type -> Type.
-    Inductive IM: type -> Type :=
-    | ITE: forall t, Term typeDenote <{{ Bool }}> ->
-                IM t ->
-                IM t ->
-                IM t
-    | RET: forall t, T t -> IM t.
-  End mvars.
+    (**
+PTerm_LTerm_rec
+     : forall (P0 : forall t : type, PTerm t -> Type) (P1 : forall t : type, LTerm t -> Type),
+       (forall p : PTerm <{{ Num }}>,
+        P0 <{{ Num }}> p ->
+        forall p0 : PTerm <{{ Num }}>, P0 <{{ Num }}> p0 -> P0 <{{ Num }}> (ADD p p0)) ->
+       (forall p : PTerm <{{ Num }}>,
+        P0 <{{ Num }}> p ->
+        forall p0 : PTerm <{{ Num }}>, P0 <{{ Num }}> p0 -> P0 <{{ Num }}> (SUB p p0)) ->
+       (forall p : PTerm <{{ Num }}>,
+        P0 <{{ Num }}> p ->
+        forall p0 : PTerm <{{ Num }}>, P0 <{{ Num }}> p0 -> P0 <{{ Num }}> (MUL p p0)) ->
+       (forall p : PTerm <{{ Num }}>,
+        P0 <{{ Num }}> p ->
+        forall p0 : PTerm <{{ Num }}>, P0 <{{ Num }}> p0 -> P0 <{{ Num }}> (DIV p p0)) ->
+       (forall (t : type) (p : PTerm <{{ Bool }}>),
+        P0 <{{ Bool }}> p ->
+        forall p0 : PTerm t, P0 t p0 -> forall p1 : PTerm t, P0 t p1 -> P0 t (ITE p p0 p1)) ->
+       (forall p : PTerm <{{ Num }}>,
+        P0 <{{ Num }}> p ->
+        forall p0 : PTerm <{{ Num }}>, P0 <{{ Num }}> p0 -> P0 <{{ Bool }}> (EQ p p0)) ->
+       (forall p : PTerm <{{ Bool }}>,
+        P0 <{{ Bool }}> p ->
+        forall p0 : PTerm <{{ Bool }}>, P0 <{{ Bool }}> p0 -> P0 <{{ Bool }}> (AND p p0)) ->
+       (forall p : PTerm <{{ Bool }}>,
+        P0 <{{ Bool }}> p ->
+        forall p0 : PTerm <{{ Bool }}>, P0 <{{ Bool }}> p0 -> P0 <{{ Bool }}> (OR p p0)) ->
+       (forall p : PTerm <{{ Bool }}>, P0 <{{ Bool }}> p -> P0 <{{ Bool }}> (NOT p)) ->
+       (forall (a : type) (l : LTerm a), P1 a l -> P0 a (L l)) ->
+       (forall f9 : Fp, P1 <{{ Num }}> (NUM f9)) ->
+       (forall b : bool, P1 <{{ Bool }}> (BOOL b)) ->
+       (forall (a b : type) (l : LTerm <{{ a -> b }}>),
+        P1 <{{ a -> b }}> l -> forall l0 : LTerm a, P1 a l0 -> P1 b (APP l l0)) ->
+       (forall (a : type) (v : var a), P1 a (VAR v)) ->
+       (forall (a b : type) (l : var a -> LTerm b),
+        (forall v : var a, P1 b (l v)) -> P1 <{{ a -> b }}> (LAM l)) ->
+       (forall (a : type) (p : PTerm a), P0 a p -> P1 a (P p)) ->
+       forall (t : type) (p : PTerm t), P0 t p
+*)
+    Scheme PTerm_LTerm_rec := Induction for PTerm Sort Type
+      with LTerm_PTerm_rec := Induction for LTerm Sort Type.
+  End pterms.
 
   Arguments VAR [var a].
   Arguments NUM {var}.
   Arguments BOOL {var}.
+  Arguments APP [var a b].
+  Arguments LAM [var a b].
+  Arguments L {var a}.
+  
   Arguments ADD {var}.
   Arguments SUB {var}.
   Arguments MUL {var}.
   Arguments DIV {var}.
+  Arguments ITE {var t}.
   Arguments EQ {var}.
   Arguments AND {var}.
   Arguments OR {var}.
-  Arguments APP [var a b].
-  Arguments LAM [var a b].
-  (** Maximally insert types in class *)
-  Arguments Nbe {var}.
-  Arguments Nbe_lam {var} {a} {b}.
-  Arguments reify {var} {t}.
-  Arguments reflect {var} {t}.
-  (** Meta terms *)
-  Arguments ITE {T t}.
-  Arguments RET {T t}.
+  Arguments NOT {var}.
+  Arguments P {var a}.
+
+  Fixpoint ptermDenote t (e: PTerm typeDenote t): typeDenote t :=
+    match e in (PTerm _ t) return (typeDenote t) with
+    | ADD a b => pkplus (ptermDenote a) (ptermDenote b)
+    | SUB a b => pksub (ptermDenote a) (ptermDenote b)
+    | MUL a b => pkmul (ptermDenote a) (ptermDenote b)
+    | DIV a b => pkdiv (ptermDenote a) (ptermDenote b)
+    | ITE c a b => if (ptermDenote c) then (ptermDenote a) else (ptermDenote b)
+    | EQ a b => if eq_field (ptermDenote a) (ptermDenote b) then true else false
+    | AND a b => andb (ptermDenote a) (ptermDenote b)
+    | OR a b => orb (ptermDenote a) (ptermDenote b)
+    | NOT a => negb (ptermDenote a)
+    | L a => ltermDenote a
+    end
+  with ltermDenote t (e : LTerm typeDenote t) {struct e} : typeDenote t :=
+    match e in (LTerm _ t) return (typeDenote t) with
+    | VAR v => v
+    | NUM f => f
+    | BOOL v => v
+    | APP e1 e2 => (ltermDenote e1) (ltermDenote e2)
+    | LAM e' => fun x => ltermDenote (e' x)
+    | P e => ptermDenote e
+    end.
+  
+  (* Normalization via reify/reflect Danvy et al. for LTerms *)
+  Class LNbe (t: type) := {
+    reify: typeDenote t -> LTerm typeDenote t;
+    reflect: LTerm typeDenote t -> typeDenote t;
+                         }.
+                                                    
+  Instance LNbe_lam {a b: type} `(LNbe a) `(LNbe b) : LNbe <{{ a -> b }}> := {
+    reify v := LAM (fun x => reify (v (reflect (VAR x))));   
+    reflect e := fun x => reflect (APP e (reify x));
+                                                                           }.
+
+  Instance LNbe_num : LNbe <{{ Num }}> := {
+    reify v := NUM v;
+    reflect v := ltermDenote v;
+                                        }.
+  
+  Instance LNbe_bool : LNbe <{{ Bool }}> := {
+    reify v := BOOL v;
+    reflect v := ltermDenote v;
+                                          }.
+  
+  (* Fine-grained normalization co-recursively in PrimaryOps terms (PTerms) and
+     Lambda Calculus terms (LTerms) *)
+  Class Nbe (t: type) := {
+    pnorm: PTerm typeDenote t -> PTerm typeDenote t;
+    lnorm: LTerm typeDenote t -> LTerm typeDenote t
+                        }.
+  
+  (* This typechecks, don't touch it! *)
+  Program Fixpoint pnorm_arr{a b: type}
+          `{LNbe <{{ a -> b }}>} `{Nbe a} `{Nbe b} `{Nbe <{{Bool}}>}
+          (e: PTerm typeDenote <{{a -> b }}>) : PTerm typeDenote <{{ a -> b }}> :=
+    match e with
+    | ITE c e1 e2 =>
+      L (LAM (fun x => P (ITE (pnorm c)
+                           (L (lnorm (APP (P (pnorm_arr e1)) (VAR x))))
+                           (L (lnorm (APP (P (pnorm_arr e2)) (VAR x)))))))
+    | L p => L (lnorm_arr p)
+    (* Bogus terms *)
+    | ADD a b => ADD a b
+    | SUB a b => SUB a b
+    | MUL a b => MUL a b
+    | DIV a b => DIV a b
+    | EQ a b => EQ a b
+    | AND a b => AND a b
+    | OR a b => OR a b
+    | NOT a => NOT a
+    end
+  with lnorm_arr{a b: type}
+                `{LNbe <{{ a -> b }}>} `{Nbe a} `{Nbe b} `{Nbe <{{Bool}}>}
+                (e: LTerm typeDenote <{{a -> b }}>) : LTerm typeDenote <{{ a -> b }}> :=
+         match e with
+         | P p => P (pnorm_arr p)
+         | APP _ _ => reify (reflect e)
+         | LAM _ => reify (reflect e)
+         | VAR _ => reify (reflect e)
+         (* Bogus terms *)
+         | NUM f => NUM f
+         | BOOL v => BOOL v
+         end.
+
+  Program Fixpoint pnorm_num(e: PTerm typeDenote <{{ Num }}>): PTerm typeDenote <{{ Num }}> :=
+      match e with
+      | ADD e1 e2 =>
+        let p1 := pnorm_num e1 in
+        let p2 := pnorm_num e2 in
+        match p1, p2 return (PTerm typeDenote <{{ Num }}>) with
+        | L (NUM n1), L (NUM n2) => L (NUM (pkplus n1 n2))
+        | _, _ => ADD p1 p2
+        end
+      | SUB e1 e2 =>
+        let p1 := pnorm_num e1 in
+        let p2 := pnorm_num e2 in
+        match p1, p2 return (PTerm typeDenote <{{ Num }}>) with
+        | L (NUM n1), L (NUM n2) => L (NUM (pksub n1 n2))
+        | _, _ => SUB p1 p2
+        end         
+      | MUL e1 e2 =>
+        let p1 := pnorm_num e1 in
+        let p2 := pnorm_num e2 in
+        match p1, p2 return (PTerm typeDenote <{{ Num }}>) with
+        | L (NUM n1), L (NUM n2) => L (NUM (pkmul n1 n2))
+        | _, _ => MUL p1 p2
+        end
+      | DIV e1 e2 =>
+        let p1 := pnorm_num e1 in
+        let p2 := pnorm_num e2 in
+        match p1, p2 return (PTerm typeDenote <{{ Num }}>) with
+        | L (NUM n1), L (NUM n2) => L (NUM (pkdiv n1 n2))
+        | _, _ => DIV p1 p2
+        end
+      | ITE c a b =>
+        let pc := pnorm_bool c in
+        match pc return (PTerm typeDenote <{{ Num }}>) with
+        | L (BOOL true) => pnorm_num a
+        | L (BOOL false) => pnorm_num b
+        | _ => ITE pc (pnorm_num a) (pnorm_num b)
+        end
+      | L a => L (lnorm_num a)
+      (* Bogus cases *)
+      | EQ a b => EQ a b
+      | AND e1 e2 => AND e1 e2
+      | OR e1 e2 => OR e1 e2
+      | NOT a => NOT a
+      end
+  with lnorm_num (e: LTerm typeDenote <{{ Num }}>): LTerm typeDenote <{{ Num }}> :=
+         match e with
+         | P p => P (pnorm_num p)
+         | APP e1 e2 => reify (reflect e)
+         | LAM _ => reify (reflect e)
+         | VAR _ => reify (reflect e)
+         | NUM f => NUM f
+         (* Bogus terms *)
+         | BOOL v => BOOL v
+         end
+  with pnorm_bool(e: PTerm typeDenote <{{ Bool }}>): PTerm typeDenote <{{ Bool }}> :=
+         match e with
+         | EQ e1 e2 =>
+           let p1 := pnorm_num e1 in
+           let p2 := pnorm_num e2 in
+           match p1, p2 return (PTerm typeDenote <{{ Bool }}>) with
+           | L (NUM n1), L (NUM n2) => L (BOOL (if eq_field n1 n2 then true else false))
+           | _, _ => EQ p1 p2
+           end
+         | AND e1 e2 => 
+           let p1 := pnorm_bool e1 in
+           let p2 := pnorm_bool e2 in
+           match p1, p2 return (PTerm typeDenote <{{ Bool }}>) with
+           | L (BOOL b1), L (BOOL b2) => L (BOOL (andb b1 b2))
+           | _, _ => AND p1 p2
+           end
+         | OR e1 e2 =>
+           let p1 := pnorm_bool e1 in
+           let p2 := pnorm_bool e2 in
+           match p1, p2 return (PTerm typeDenote <{{ Bool }}>) with
+           | L (BOOL b1), L (BOOL b2) => L (BOOL (orb b1 b2))
+           | _, _ => OR p1 p2
+           end
+         | NOT a =>
+           let p1 := pnorm_bool a in
+           match p1 return (PTerm typeDenote <{{ Bool }}>) with
+           | L (BOOL b1) => L (BOOL (negb b1))
+           | _ => NOT p1
+           end
+         | L a => L (lnorm_bool a)
+         | ITE c a b =>
+           let pc := pnorm_bool c in
+           match pc return (PTerm typeDenote <{{ Bool }}>) with
+           | L (BOOL true) => pnorm_bool a
+           | L (BOOL false) => pnorm_bool b
+           | _ => ITE pc (pnorm_bool a) (pnorm_bool b)
+           end
+         (* Bogus patterns *)
+         | ADD a b => ADD a b
+         | SUB a b => SUB a b
+         | MUL a b => MUL a b
+         | DIV a b => DIV a b
+         end
+  with lnorm_bool (e: LTerm typeDenote <{{ Bool }}>): LTerm typeDenote <{{ Bool }}> :=
+         match e with
+         | P p => P (pnorm_bool p)
+         | APP e1 e2 => reify (reflect e)
+         | LAM _ => reify (reflect e)
+         | VAR _ => reify (reflect e)
+         | BOOL v => BOOL v
+         (* Bogus terms *)
+         | NUM f => NUM f
+         end.
+  
+  Instance Nbe_num : Nbe <{{ Num }}> := {
+    pnorm := pnorm_num;
+    lnorm := lnorm_num;
+    }.
+
+  Instance Nbe_bool: Nbe <{{ Bool }}> := {
+    pnorm := pnorm_bool;
+    lnorm := lnorm_bool
+                                        }.
+
+                                                     
+  Instance Nbe_lam {a b: type} `(Nbe a) `(Nbe b) `(LNbe <{{ a -> b }}>): Nbe <{{ a -> b }}> := {
+    pnorm := pnorm_arr;
+    lnorm := lnorm_arr
+                                                                                            }.
   
   Declare Custom Entry stlc.
   Notation "'fp' n" := (NUM n) (in custom stlc at level 0).
@@ -179,72 +374,10 @@ Module Stlc(Import PF: GaloisField.GaloisField).
                     y custom stlc at level 99,
                     z custom stlc at level 99,
                     left associativity).  
-  
-  Fixpoint termDenote t (e : Term typeDenote t) {struct e} : typeDenote t :=
-    match e in (Term _ t) return (typeDenote t) with
-    | VAR v => v
-    | NUM f => f
-    | BOOL v => v
-    | ADD f1 f2 => pkplus (termDenote f1) (termDenote f2)
-    | SUB f1 f2 => pksub (termDenote f1) (termDenote f2)
-    | MUL f1 f2 => pkmul (termDenote f1) (termDenote f2)
-    | DIV f1 f2 => pkdiv (termDenote f1) (termDenote f2)
-    | EQ f1 f2 => if eq_field (termDenote f1) (termDenote f2) then true else false
-    (** Commuting conversion if/app *)
-    (* | @ITE _ <{{ a -> b }}> c t e =>
-      fun y => if (termDenote c) then (termDenote t) y else (termDenote e) y
-    | ITE c t e => if (termDenote c) then termDenote t else termDenote e *)
-    | AND b1 b2 => andb (termDenote b1) (termDenote b2)
-    | OR b1 b2 => orb (termDenote b1) (termDenote b2)
-    | NOT b => negb (termDenote b)
-    | APP e1 e2 => (termDenote e1) (termDenote e2)
-    | LAM e' => fun x => termDenote (e' x)
-    end.
 
+  Coercion P: PTerm >-> LTerm.
+  Coercion L: LTerm >-> PTerm.
 
-  Fixpoint mtermDenote t (e: IM (Term typeDenote) t) : typeDenote t :=
-    match e with
-    | ITE c e1 e2 => if (termDenote c) then (mtermDenote e1) else mtermDenote e2
-    | RET e => termDenote e
-    end.  
-  
-  Instance Nbe_int : Nbe <{{ Num }}> := {
-    reify v := NUM v;
-    reflect v := termDenote v;
-                                }.
-
-  Instance Nbe_bool : Nbe <{{ Bool }}> := {
-    reify v := BOOL v;
-    reflect v := termDenote v;
-                                  }.
-
-  Fixpoint resolver(t: type): Nbe t :=
-    match t with
-    | <{{ Bool }}> => Nbe_bool
-    | <{{ Num }}> => Nbe_int
-    | <{{ a -> b }}> => Nbe_lam (resolver a) (resolver b)
-    end.
-
-  (** This function does *partial* reflection of the object language while
-      maintaining the syntax of the metalanguage! *)
-  Fixpoint mreflect t (e: IM (Term typeDenote) t): IM typeDenote t :=
-    match e with
-    | @ITE _ <{{ a -> b }}> c e1 e2 =>
-      
-    | ITE c e1 e2 =>
-      ITE (BOOL (reflect (resolver <{{ Bool }}>) c))
-          (mreflect e1) (mreflect e2)
-    | RET e => RET (reflect (resolver _) e)
-    end.
-
-  (** Conversely, this function is dumb and uninteresting. Since we cannot
-      reify if-then-else statements from Gallina to IM *)
-  Definition mreify{t: type} (e: typeDenote t): IM (Term typeDenote) t :=
-    RET (reify (resolver t) e).
-
-  Definition normalize {t: type} (e: Term typeDenote t) : Term typeDenote t :=
-    reif (refl e).
-                                       
   Inductive fof: type -> Prop :=
   | fo_bool: fof <{{ Bool }}>
   | fo_num: fof <{{ Num }}>
@@ -255,14 +388,14 @@ Module Stlc(Import PF: GaloisField.GaloisField).
       fof <{{ a }}> ->
       fof <{{ Num -> a }}>.
 
-  Inductive value: forall (t: type), Term typeDenote t -> Prop :=
+  Inductive value: forall (t: type), LTerm typeDenote t -> Prop :=
   | Value_bool: forall x, @value <{{ Bool }}> (@VAR typeDenote <{{ Bool }}> x)
   | Value_btrue: @value <{{ Bool }}> <{ true }>
   | Value_bfalse: @value <{{ Bool }}> <{ false }>
   | Value_var: forall x, @value <{{ Num }}> (@VAR typeDenote <{{ Num }}> x)
   | Value_const: forall (x: Fp), @value <{{ Num }}> (NUM x).
   
-  Inductive hnff: forall (t: type), Term typeDenote t -> Prop :=
+  Inductive hnff: forall (t: type), LTerm typeDenote t -> Prop :=
   | HNF_bool_ar: forall a f,
       (forall (arg: typeDenote <{{ Bool }}>), @hnff <{{ a }}> (f arg)) ->
       @hnff <{{ Bool -> a }}> (LAM f)
@@ -276,13 +409,31 @@ Module Stlc(Import PF: GaloisField.GaloisField).
       value e ->
       @hnff <{{ Num }}> e.
 
+  (* Undecidable instance resolution sucks *)
+  Fixpoint resolver(t: type): Nbe t :=
+    match t with
+    | <{{ Bool }}> => Nbe_bool
+    | <{{ Num }}> => Nbe_num
+    | <{{ a -> b }}> => Nbe_lam (resolver a) (resolver b)
+                              (LNbe_lam (lresolver a) (lresolver b))
+    end
+  with lresolver(t: type): LNbe t :=
+    match t with
+    | <{{ Bool }}> => LNbe_bool
+    | <{{ Num }}> => LNbe_num
+    | <{{ a -> b }}> => LNbe_lam (lresolver a) (lresolver b)
+    end.
+
+  Definition normalize t (e: LTerm typeDenote t): LTerm typeDenote t :=
+    @lnorm t (resolver t) e.
+  
   (** Provide default witnesses for hnff *)
   (* Hint Extern 3 (typeDenote <{{ Bool }}>) => exact (true).
   Hint Extern 3 (typeDenote <{{ Num }}>) => exact (0:%p).
   *)
-  Theorem normalize_correct: forall (t: type) (e: Term typeDenote t),
+  Theorem normalize_correct: forall (t: type) (e: LTerm typeDenote t),
       fof t  -> 
-      @hnff t (@normalize t e).
+      @hnff t (normalize e).
   Proof with eauto.
     intros.
     generalize dependent e.
@@ -290,23 +441,16 @@ Module Stlc(Import PF: GaloisField.GaloisField).
     induction t; intros; dependent destruction e; cbn; try constructor;
       invert H; cbn; try constructor...
     - destruct b; constructor.
-    - destruct (eq_field (termDenote e1) (termDenote e2)); constructor.
-    - destruct (termDenote e1); destruct (termDenote e2); constructor.
-    - destruct (termDenote e1); destruct (termDenote e2); constructor.
-    - destruct (termDenote e); constructor.
-    - destruct (termDenote e1); destruct (termDenote e2); destruct (termDenote e3); constructor.
-    - destruct ((termDenote e1 (termDenote e2))); constructor.
+    - destruct (ltermDenote e1); constructor. 
     - destruct t; constructor.
-  Defined.
+    - admit.  
+    - admit. 
+  Admitted.
 
-
-  Definition t: Term typeDenote <{{ Bool -> Bool }}> :=
+  Definition t: LTerm typeDenote <{{ Bool -> Bool }}> :=
     <{ \x, (if # x then \y, # y else \z, ! # z) # x }>.
   
   Eval cbv in normalize t.
-
-  Eval cbv in reflect (resolver _) (reify (resolver <{{ Bool -> Bool }}>) f).
-  Eval cbv in reflect (resolver _) (normalize t) true.
 
   Example notnormal: @hnff <{{ Bool -> Bool }}> (normalize t).
   Proof.
